# Table of Contents
- [Derivative formulas](#derivative-formulas)
  - [Power Rule examples](#power-rule-examples)
  - [General Power Rule](#general-power-rule)
  - [Derivative of 1/x](#derivative-of-1x)
  - [Derivative of sqrt(x)](#derivative-of-sqrtx)
  - [Derivative of sin(theta)](#derivative-of-sintheta)
  - [Derivative of Exponential Functions](#derivative-of-exponential-functions)

---

### Derivative formulas:

- for function f(x) = x¬≤  
It gives an upward parabola  

![parabola](./images/d_formula1.png)

Here dx¬≤ is very tiny amount ‚Üí negligible

- For f(x) = x¬≥  

![cube-volume-change](./images/d_formula2.png)

- When x is changed a little bit, the volume also get changed
- Here the small cubes and side rectangles can be neglected as they are very small in actual computation
- Only 3 squared volumes are considere
- Thus it becomes 3 x¬≤ dx (l*b*h)
- df/dx ‚Üí divided by dx, all the dx terms will get discarded here

<aside>
üí°

In general way,  
**d (x‚Åø) / dx = nx‚Åø‚Åª¬π**

This is known as ‚Äú**Power Rule**‚Äù

</aside>

![power-rule-proof](./images/d_formula3.png)

Small change dx added to x, f(x+dx) = (x+dx)‚Åø

- d(f(x)) = f(x+dx) - f(x)  
And this will get divided by dx on both sides  
Thus, x‚Åø and dx terms get reduced

---

- f(x) = 1/x  
    - Here,
        f(1) = 1  
        f(2) = 0.5  
        f(3) = 0.33  
    - The area is 1  

![hyperbola-area](./images/d_formula4.png)

        Can be found in 2 ways,

![method-1](./images/d_formula5.jpg)

(or)

![method-2](./images/d_formula6.jpg)

---

- f(x) = sqrt(x)

![sqrt-graph](./images/d_formula7.jpg)

[]()

---

- f(theta) = sin(theta)

![sine-curve](./images/d_formula8.png)

Here d(sin(theta)) / d(theta) = slope of this graph

![sine-slope](./images/d_formula9.png)

Consider a small change in theta, this increases the sin(theta)

![sine-small-change](./images/d_formula10.png)

---

# Derivative of exponent

![exponential-derivative](./images/d_formula11.jpg)

- this constant will get added on for any x^t
- The constant is directly proportional to x
- This constant will be 1 when x=e (Euler number)

**Derivative of e^x = e^x**

**Derivative of e^(cx) = c e^(cx), where c is constant (by chain rule)**

$$
x = e^{(\ln(x))}
$$

From this,

$$
\frac{d}{dt}\left(2^t\right) = \frac{d}{dt}\left(e^{(\ln 2)t}\right)
$$

We know that,

$$
\frac{d}{dt}\left(e^{ct}\right) = c e^{ct}
$$

By applying,

$$
\frac{d}{dt}\left(e^{(\ln 2)t}\right)
= (\ln 2)\, e^{(\ln 2)t}
\\
(\ln 2)\, e^{(\ln 2)t} = (\ln 2)\, 2^t
\\
\frac{d}{dt}\left(2^t\right) = (\ln 2)\, 2^t
$$
